#### Aufgabe 3:
a) $$\begin{align}\int_{0}^{4}x^{2}\,dx&=\bigg[\frac{1}{3}x^{3}\bigg]_{0}^{4}\\
&=\left(\frac{1}{3}\cdot4^{3}\right)-\left(\frac{1}{3}\cdot0^{3}\right)\\
&=\frac{64-0}{3}\\
&=21,\overline{3}\end{align}$$
b) $$\begin{align}\int_{2}^{4}x^{2}\,dx&=\bigg[\frac{1}{3}x^{3}\bigg]_{2}^{4}\\
&=\left(\frac{1}{3}\cdot4^{3}\right)-\left(\frac{1}{3}\cdot2^{3}\right)\\
&=\frac{64-8}{3}\\
&=18,\overline{6}\end{align}$$
c) $$\begin{align}\int_{-1}^{5}2x\,dx&=\bigg[x^{2}\bigg]_{-1}^{5}\\
&=\left(5^{2}\right)-\left((-1)^{2}\right)\\
&={15-1}\\
&=24\end{align}$$
d) $$\begin{align}\int_{10}^{11}0,5x\,dx&=\bigg[\frac{1}{4}x^{2}\bigg]_{10}^{11}\\
&=\left(\frac{1}{4}\cdot11^{2}\right)-\left(\frac{1}{4}\cdot10^{2}\right)\\
&=\frac{121-100}{4}\\
&=5,25\end{align}$$
e) $$\begin{align}\int_{10}^{20}5\,dx&=\bigg[{5}x\bigg]_{10}^{20}\\
&=\left(5\cdot20\right)-\left(5\cdot10\right)\\
&={100-50}\\
&=50\end{align}$$
f) $$\begin{align}\int_{0}^{1}x^{3}\,dx&=\bigg[\frac{1}{4}x^{4}\bigg]_{0}^{1}\\
&=\left(\frac{1}{4}\cdot1^{4}\right)-\left(\frac{1}{4}\cdot0^{4}\right)\\
&=\frac{1-0}{4}\\
&=0,25\end{align}$$
g) $$\begin{align}\int_{0}^{3}0,5x^{2}\,dx&=\bigg[\frac{1}{6}x^{3}\bigg]_{0}^{3}\\
&=\left(\frac{1}{6}\cdot3^{3}\right)-\left(\frac{1}{6}\cdot0^{3}\right)\\
&=\frac{27-0}{6}\\
&=4,5\end{align}$$
h) $$\begin{align}\int_{-2}^{0}\frac{1}{3}x^{3}\,dx&=\bigg[\frac{1}{12}x^{4}\bigg]_{-2}^{0}\\
&=\left(\frac{1}{12}\cdot0^{4}\right)-\left(\frac{1}{12}\cdot(-2)^{4}\right)\\
&=\frac{0-16}{12}\\
&=-1\frac{1}{4}\\
&=-1,25\end{align}$$
i) $$\begin{align}\int_{-2}^{-1}\frac{1}{8}x^{4}\,dx&=\bigg[\frac{1}{40}x^{5}\bigg]_{-2}^{-1}\\
&=\left(\frac{1}{40}\cdot(-2)^{5}\right)-\left(\frac{1}{40}\cdot(-1)^{5}\right)\\
&=\frac{-(32)-(-1)}{40}\\
&=0,775\end{align}$$
j) $$\begin{align}\int_{-4}^{4}0,5x^{2}\,dx&=\bigg[\frac{1}{6}x^{3}\bigg]_{-4}^{4}\\
&=\left(\frac{1}{6}\cdot4^{3}\right)-\left(\frac{1}{6}\cdot(-4)^{3}\right)\\
&=\frac{64-(-64)}{6}\\
&=21,\overline{6}\end{align}$$
k) $$\begin{align}\int_{-1}^{1}x^{5}\,dx&=\bigg[\frac{1}{6}x^{6}\bigg]_{-1}^{1}\\
&=\left(\frac{1}{6}\cdot1^{6}\right)-\left(\frac{1}{6}\cdot(-1)^{6}\right)\\
&=\frac{1-(-1)}{6}\\
&=1,1\overline{6}\end{align}$$
l) $$\begin{align}\int_{90}^{100}1\,dx&=\bigg[x\bigg]_{90}^{100}\\
&=\left(100\right)-\left(90\right)\\
&={100-90}\\
&=10\end{align}$$







