---
aliases:
  - 25.04.2024 h
---
$$
\begin{align}
	\begin{pmatrix}n\\d-k\end{pmatrix}
	\cdot p^{d-k}\cdot{(1-p)}^{n-(d-k)}&=\begin{pmatrix}n\\d-k\end{pmatrix}
	\cdot p^{(d-k)}\cdot (1-p)^{n-(d+k)} \\
	
	\begin{pmatrix}10\\5-k\end{pmatrix}
	\cdot 0,5^{(5-k)}\cdot{(1-0,5)}^{10-(5-k)}&=\begin{pmatrix}n\\5+k\end{pmatrix}
	\cdot 0,5^{(5+k)}\cdot (1-0,5)^{10-(5+k)} \\
		
	\frac{10!}{(10-(5-k))!\cdot(5-k)!}
	\cdot 0,5^5\cdot0,5^{(-k)}\cdot0,5^{10-5+k}
	&=
	\frac{10!}{(10-(5+k))!\cdot(5+k)!}
	\cdot 0,5^5\cdot0,5^{-k}\cdot0,5^{10-5-k}\\
		
	\frac{10!}{(10-(5-k))!\cdot(5-k)!}
	\cdot 0,5^5\cdot0,5^{-k}\cdot \frac{0,5^{10}\cdot0,5^{k}}{0,5^{5}}
	&=
	\frac{10!}{(10-(5+k))!\cdot(5+k)!}
	\cdot 0,5^5\cdot0,5^k\cdot \frac{0,5^{10}\cdot0,5^{k}}{0,5^{5}} \\
		
	\frac{10!}{(10-(5-k))!\cdot(5-k)!}
	\cdot \cancel{0,5^5}\cdot\cancel{0,5^{-k}}\cdot \frac{0,5^{10}}{\cancel{0,5^{5}}\cdot\cancel{0,5^{k}}}
	&=
	\frac{10!}{(10-(5+k))!\cdot(5+k)!}
	\cdot \cancel{0,5^5}\cdot\cancel{0,5^k}\cdot \frac{0,5^{10}}{\cancel{0,5^5}\cdot\cancel{0,5^{k}}} \\
		
	\frac{10!}{(10-5+k)!\cdot(5-k)!}
	\cdot 0,5^{10}
	&=
	\frac{10!}{(10-5-k)!\cdot(5+k)!}
	\cdot 0,5^{10}\\
		
	\frac{10!}{(5+k)!\cdot(5-k)!}
	\cdot 0,5^{10}
	&=
	\frac{10!}{(5-k)!\cdot(5+k)!}
	\cdot 0,5^{10} 
	&&\mid :0,5^{10}\\
		
	\frac{10!}{(5+k)!\cdot(5-k)!}
	&=
	\frac{10!}{(5-k)!\cdot(5+k)!}
	&&\mid \cdot(5+k)!\\
		
	\frac{10!}{(5-k)!}
	&=
	\frac{10!}{(5-k)!}
	&&\mid \cdot(5-k)! \\
		
	10!
	&=
	10!
	&&\mid :10! \\
		
	1
	&=
	1
\end{align}
$$

