### Buch Seite 235
###### Aufgabe 1:
###### a) $$\begin{align}
\vec{AB}&=\left(\begin{matrix}
2 \\
1 \\
3
\end{matrix}\right) \\
|\vec{AB}|&=\sqrt{ 2^2 + 1^2 +3^2 } \\
|\vec{AB}|&=3,810.249.676
\end{align}$$
###### b) $$\begin{align}
\vec{AB}&=\left(\begin{matrix}
3 \\
- 6\\
-4
\end{matrix}\right) \\
|\vec{AB}|&=\sqrt{ 3^2 + (-6)^2 +(-4)^2 } \\
|\vec{AB}|&=7,681.145.748
\end{align}$$
###### c) $$\begin{align}
\vec{AB}&=\left(\begin{matrix}
8 \\
- 2\\
-5
\end{matrix}\right) \\
|\vec{AB}|&=\sqrt{ 8^2 + (-2)^2 (-5)^2 } \\
|\vec{AB}|&=9,643.650.761
\end{align}$$
---
### Buch Seite 236
##### Aufgabe 2:
###### a) $$\begin{align}
\vec{a}&=\left(\begin{matrix}
1 \\
0\\
2
\end{matrix}\right) \\
|\vec{a}|&=\sqrt{ 1^2 + 0^2 +2^2 } \\
|\vec{a}|&=2,236.067.977 \\
\vec{e_{v}}&=\left(\begin{matrix}
\frac{1}{2,236.067.977} \\
\frac{0}{2,236.067.977}\\
\frac{2}{2,236.067.977}
\end{matrix}\right)
\end{align}$$
###### b)$$\begin{align}
\vec{b}&=\left(\begin{matrix}
3\\
-2\\
1
\end{matrix}\right) \\
|\vec{b}|&=\sqrt{ 3^2 + â€”2)^2 +1^2 } \\
|\vec{b}|&=3,741.657.387\\
\vec{e_{v}}&=\left(\begin{matrix}
\frac{1}{3,741.657.387} \\
\frac{0}{3,741.657.387}\\
\frac{2}{3,741.657.387}
\end{matrix}\right)
\end{align}$$
###### c) $$\begin{align}
\vec{c}&=\left(\begin{matrix}
0 \\
-1\\
0
\end{matrix}\right) \\
|\vec{c}|&=\sqrt{ 0^2 + (-1)^2 +0^2 } \\
|\vec{c}|&=1 \\
\vec{e_{v}}&=\left(\begin{matrix}
\frac{1}{1} \\
\frac{0}{1}\\
\frac{2}{1}
\end{matrix}\right)
\end{align}$$
###### d) $$\begin{align}
\vec{d}&=\left(\begin{matrix}
0,2 \\
0,2\\
2,1
\end{matrix}\right) \\
|\vec{d}|&=\sqrt{ 0,2^2 + 0,2^2 +0,1^2 } \\
|\vec{d}|&=0,3 \\
\vec{e_{v}}&=\left(\begin{matrix}
\frac{1}{0,3} \\
\frac{0}{0,3}\\
\frac{2}{0,3}
\end{matrix}\right)
\end{align}$$
###### e) $$\begin{align}
\vec{e}&=\left(\begin{matrix}
\sqrt{ 2 } \\
\sqrt{ 3 }\\
\sqrt{ 5 }
\end{matrix}\right) \\
|\vec{e}|&=\sqrt{ (\sqrt{ 2 })^2 + (\sqrt{ 3 })^2 +(\sqrt{ 5 })^2 } \\
|\vec{e}|&=\sqrt{ (2)^{2/2} + (3 )^{2/2} +( 5 )^{2/2} } \\
|\vec{e}|&=\sqrt{ (2) + (3 ) +( 5 ) } \\
|\vec{e}|&=3,162.277.66 \\
\vec{e_{v}}&=\left(\begin{matrix}
\frac{1}{3,162.277.66} \\
\frac{0}{3,162.277.66}\\
\frac{2}{3,162.277.66}
\end{matrix}\right)
\end{align}$$
###### f)$$\begin{align}
\vec{f}&=\frac{1}{4}\left(\begin{matrix}
3 \\
1\\
4
\end{matrix}\right) \\
\vec{f}&=\left(\begin{matrix}
\frac{3}{4} \\
\frac{1}{4}\\
\frac{4}{4}
\end{matrix}\right) \\
|\vec{f}|&=\sqrt{ \frac{3}{4}^2 + \frac{1}{4}^2 +\frac{4}{4}^2 } \\
|\vec{f}|&=1,274.754.878 \\
\vec{e_{v}}&=\left(\begin{matrix}
\frac{1}{1,274.754.878} \\
\frac{0}{1,274.754.878}\\
\frac{2}{1,274.754.878}
\end{matrix}\right)
\end{align}$$
###### g) $$\begin{align}
\vec{g}&=0,1\left(\begin{matrix}
4 \\
3\\
0
\end{matrix}\right) \\
\vec{g}&=\left(\begin{matrix}
0,4 \\
0,3\\
0,0
\end{matrix}\right) \\
|\vec{g}|&=\sqrt{ (0,4)^2 + (0,3)^2 +(0,0)^2 } \\
|\vec{g}|&=0,5 \\
\vec{e_{v}}&=\left(\begin{matrix}
\frac{1}{0,5} \\
\frac{0}{0,5}\\
\frac{2}{0,5}
\end{matrix}\right)
\end{align}$$
---
##### Aufgabe 3:

$$\left( \begin{matrix}
a_{2}b_{3}-a_{3}b_{2} \\
a_{3}b_{1}-a_{1}b_{3} \\
a_{1}b_{2}-a_{2}b_{1} \\
\end{matrix}\right)
$$
###### a)$$\begin{align}
\vec{a}=\left(\begin{matrix}
1 \\
0 \\
0
\end{matrix}\right)&\quad\vec{b}=\left(\begin{matrix}
3 \\
2 \\
4
\end{matrix}\right) \\
\vec{a}=\left(\begin{matrix}
1 \\
0 \\
0
\end{matrix}\right)&\times\vec{b}=\left(\begin{matrix}
3 \\
2 \\
4
\end{matrix}\right) \\
\left( \begin{matrix}
0_{2}4_{3}-0_{3}2_{2} \\
0_{3}3_{1}-1_{1}4_{3} \\
1_{1}2_{2}-0_{2}3_{1} \\
\end{matrix}\right) \\
\left( \begin{matrix}
0 \\
- 4\\
 2\\
\end{matrix}\right)
\end{align}$$
###### b)$$\begin{align}
\vec{a}=\left(\begin{matrix}
1 \\
0 \\
0
\end{matrix}\right)&\quad\vec{b}=\left(\begin{matrix}
3 \\
2 \\
4
\end{matrix}\right) \\
\vec{a}=\left(\begin{matrix}
1 \\
0 \\
0
\end{matrix}\right)&\times\vec{b}=\left(\begin{matrix}
3 \\
2 \\
4
\end{matrix}\right) \\
\left(\begin{array}{rrr} &\begin{matrix} 0\cdot3 \\ 1\cdot4 \\ 1\cdot2 \end{matrix} &\begin{matrix} -\\ -\\ - \end{matrix} &\begin{matrix} 0\cdot2 \\ 1\cdot4 \\ 0\cdot3 \end{matrix} \end{array} \right) \\
\left( \begin{matrix}
0 \\
- 4\\
 2\\
\end{matrix}\right)
\end{align}$$


$$\left( \begin{matrix}
0_{2}4_{3}-0_{3}2_{2} \\
0_{3}3_{1}-1_{1}4_{3} \\
1_{1}2_{2}-0_{2}3_{1} \\
\end{matrix}\right)$$

$$\begin{align} &\left( \begin{matrix} 0\cdot3 \\ 1\cdot4 \\ 1\cdot2 \end{matrix} &\begin{matrix} -\\ -\\ - \end{matrix} &\begin{matrix} 0\cdot2 \\ 1\cdot4 \\ 0\cdot3 \end{matrix} \right)\end{align}$$

$$\left(\begin{array}{rrr} &\begin{matrix} 0\cdot3 \\ 1\cdot4 \\ 1\cdot2 \end{matrix} &\begin{matrix} -\\ -\\ - \end{matrix} &\begin{matrix} 0\cdot2 \\ 1\cdot4 \\ 0\cdot3 \end{matrix} \end{array} \right)$$




$$\left( \begin{matrix} 0\cdot3 \\ 1\cdot4 \\ 1\cdot2 \end{matrix} \begin{matrix} -\\ -\\ - \end{matrix} \begin{matrix} 0\cdot2 \\ 1\cdot4 \\ 0\cdot3 \end{matrix} \right)$$
